src/dvspec/dafny/att_spec_proofs/dvn_next_invs_8_18.dfy
@@ -1,0 +1,331 @@
+include "../commons.dfy"
+include "../specification/dvc_spec.dfy"
+include "../specification/consensus.dfy"
+include "../specification/network.dfy"
+include "../specification/dvn.dfy"
+include "../att_spec_proofs/inv.dfy"
+include "../att_spec_proofs/assump.dfy"
+include "../att_spec_proofs/fnc_inv.dfy"
+include "../att_spec_proofs/helper_sets_lemmas.dfy"
+include "../att_spec_proofs/proofs_intermediate_steps.dfy"
+include "../att_spec_proofs/dvn_next_invs_1_7.dfy"
+
+module DVN_Next_Invs_8_18
+{
+    import opened Types 
+    import opened CommonFunctions
+    import opened ConsensusSpec
+    import opened NetworkSpec
+    import opened DVCNode_Spec
+    import opened DV
+    import opened Att_Inv_With_Empty_Initial_Attestation_Slashing_DB
+    import opened Att_Assumptions
+    import opened Fnc_Inv
+    import opened Helper_Sets_Lemmas
+    import opened Proofs_Intermediate_Steps
+    import opened DVN_Next_Invs_1_7
+
+     
+
+    lemma lemma_inv8_dvn_next(
+        dvn: DVState,
+        event: DV.Event,
+        dvn': DVState
+    )    
+    requires NextEvent(dvn, event, dvn')    
+    requires inv8(dvn)
+    ensures inv8(dvn')
+    {        
+        match event 
+        {
+            case HonestNodeTakingStep(node, nodeEvent, nodeOutputs) =>
+                var dvc := dvn.honest_nodes_states[node];
+                var dvc' := dvn'.honest_nodes_states[node];
+                assert inv8_body(dvc);
+                match nodeEvent
+                {
+                    case ServeAttstationDuty(attestation_duty) =>                             
+                        lemma_inv8_f_serve_attestation_duty(dvc, attestation_duty, dvc');
+                        
+                    case AttConsensusDecided(id, decided_attestation_data) => 
+                        lemma_inv8_f_att_consensus_decided(dvc, id, decided_attestation_data, dvc');                                                
+                        
+                    case ReceviedAttesttionShare(attestation_share) =>                         
+                        lemma_inv8_f_listen_for_attestation_shares(dvc, attestation_share, dvc');                        
+   
+                    case ImportedNewBlock(block) => 
+                        var dvc_mod := add_block_to_bn(dvc, nodeEvent.block);
+                        lemma_inv8_add_block_to_bn(dvc, nodeEvent.block, dvc_mod);
+                        assert inv8_body(dvc_mod);
+                        lemma_inv8_f_listen_for_new_imported_blocks(dvc_mod, block, dvc');                        
+                        assert inv8_body(dvc');
+                        
+                    case ResendAttestationShares =>                                                                      
+
+                    case NoEvent => 
+                        
+                }
+
+            case AdeversaryTakingStep(node, new_attestation_share_sent, messagesReceivedByTheNode) =>
+                
+        }   
+    }  
+
+    lemma lemma_inv9_dvn_next(
+        dvn: DVState,
+        event: DV.Event,
+        dvn': DVState
+    )    
+    requires NextEvent(dvn, event, dvn')    
+    requires inv9(dvn)
+    ensures inv9(dvn')
+    {        
+        match event 
+        {
+            case HonestNodeTakingStep(node, nodeEvent, nodeOutputs) =>
+                var dvc := dvn.honest_nodes_states[node];
+                var dvc' := dvn'.honest_nodes_states[node];
+                assert inv9_body(dvc);
+                match nodeEvent
+                {
+                    case ServeAttstationDuty(attestation_duty) =>                             
+                        lemma_inv9_f_serve_attestation_duty(dvc, attestation_duty, dvc');
+                        
+                    case AttConsensusDecided(id, decided_attestation_data) => 
+                        lemma_inv9_f_att_consensus_decided(dvc, id, decided_attestation_data, dvc');                                                
+                        
+                    case ReceviedAttesttionShare(attestation_share) =>                         
+                        lemma_inv9_f_listen_for_attestation_shares(dvc, attestation_share, dvc');                        
+   
+                    case ImportedNewBlock(block) => 
+                        var dvc_mod := add_block_to_bn(dvc, nodeEvent.block);
+                        lemma_inv9_add_block_to_bn(dvc, nodeEvent.block, dvc_mod);
+                        assert inv9_body(dvc_mod);
+                        lemma_inv9_f_listen_for_new_imported_blocks(dvc_mod, block, dvc');                        
+                        assert inv9_body(dvc');
+                        
+                    case ResendAttestationShares =>                                                                      
+
+                    case NoEvent => 
+                        
+                }
+
+            case AdeversaryTakingStep(node, new_attestation_share_sent, messagesReceivedByTheNode) =>
+                
+        }   
+    }  
+
+    lemma lemma_inv10_dvn_next(
+        dvn: DVState,
+        event: DV.Event,
+        dvn': DVState
+    )    
+    requires NextEvent(dvn, event, dvn')        
+    requires inv10(dvn)
+    ensures inv10(dvn')
+    {        
+        match event 
+        {
+            case HonestNodeTakingStep(node, nodeEvent, nodeOutputs) =>
+                var dvc := dvn.honest_nodes_states[node];
+                var dvc' := dvn'.honest_nodes_states[node];
+                assert inv10_body(dvc);
+                match nodeEvent
+                {
+                    case ServeAttstationDuty(attestation_duty) =>                             
+                        lemma_inv10_f_serve_attestation_duty(dvc, attestation_duty, dvc');
+                        
+                    case AttConsensusDecided(id, decided_attestation_data) => 
+                        lemma_inv10_f_att_consensus_decided(dvc, id, decided_attestation_data, dvc');                                                
+                        
+                    case ReceviedAttesttionShare(attestation_share) =>                         
+                        lemma_inv10_f_listen_for_attestation_shares(dvc, attestation_share, dvc');                        
+   
+                    case ImportedNewBlock(block) => 
+                        var dvc_mod := add_block_to_bn(dvc, nodeEvent.block);
+                        lemma_inv10_add_block_to_bn(dvc, nodeEvent.block, dvc_mod);
+                        assert inv10_body(dvc_mod);
+                        lemma_inv10_f_listen_for_new_imported_blocks(dvc_mod, block, dvc');                        
+                        assert inv10_body(dvc');
+                        
+                    case ResendAttestationShares =>                                                                      
+
+                    case NoEvent => 
+                        
+                }
+
+            case AdeversaryTakingStep(node, new_attestation_share_sent, messagesReceivedByTheNode) =>
+                
+        }   
+    }  
+
+    
+    lemma lemma_inv13_dvn_next(
+        dvn: DVState,
+        event: DV.Event,
+        dvn': DVState
+    )    
+    requires NextEvent(dvn, event, dvn')    
+    requires inv13(dvn)
+    ensures inv13(dvn)
+    { }
+    
+
+    // It takes more than 60 seconds to prove lemma_inv16_dvn_next.
+    lemma lemma_inv16_dvn_next(
+        dvn: DVState,
+        event: DV.Event,
+        dvn': DVState
+    )    
+    requires NextEvent(dvn, event, dvn')    
+    requires inv8(dvn)
+    requires inv16(dvn)
+    ensures inv16(dvn')
+    {        
+        match event 
+        {
+            case HonestNodeTakingStep(node, nodeEvent, nodeOutputs) =>
+                var dvc := dvn.honest_nodes_states[node];
+                var dvc' := dvn'.honest_nodes_states[node];
+                assert inv16_body(dvc);
+                match nodeEvent
+                {
+                    case ServeAttstationDuty(attestation_duty) =>                             
+                        lemma_inv16_f_serve_attestation_duty(dvc, attestation_duty, dvc');
+                        
+                    case AttConsensusDecided(id, decided_attestation_data) => 
+                        lemma_inv16_f_att_consensus_decided(dvc, id, decided_attestation_data, dvc');                                                
+                        
+                    case ReceviedAttesttionShare(attestation_share) =>                         
+                        lemma_inv16_f_listen_for_attestation_shares(dvc, attestation_share, dvc');                        
+   
+                    case ImportedNewBlock(block) => 
+                        var dvc_mod := add_block_to_bn(dvc, nodeEvent.block);
+                        lemma_inv16_add_block_to_bn(dvc, nodeEvent.block, dvc_mod);
+                        assert inv16_body(dvc_mod);
+                        lemma_inv16_f_listen_for_new_imported_blocks(dvc_mod, block, dvc');                        
+                        assert inv16_body(dvc');
+                        
+                    case ResendAttestationShares =>                                                                      
+
+                    case NoEvent => 
+                        
+                }
+
+            case AdeversaryTakingStep(node, new_attestation_share_sent, messagesReceivedByTheNode) =>
+                
+        }   
+    }  
+
+    lemma lemma_inv17_dvn_next(
+        dvn: DVState,
+        event: DV.Event,
+        dvn': DVState
+    )    
+    requires NextEvent(dvn, event, dvn')  
+    requires inv1(dvn)  
+    requires inv2(dvn)
+    requires inv4(dvn)
+    requires inv5(dvn)
+    requires inv13(dvn)
+    requires inv15(dvn)
+    requires inv17(dvn)
+    ensures inv17(dvn')
+    {        
+        match event 
+        {
+            case HonestNodeTakingStep(node, nodeEvent, nodeOutputs) =>
+                var dvc := dvn.honest_nodes_states[node];
+                var dvc' := dvn'.honest_nodes_states[node];
+                
+                
+                match nodeEvent
+                {
+                    case ServeAttstationDuty(attestation_duty) =>                                                                     
+                        lemma_inv17_f_serve_attestation_duty(dvc, attestation_duty, dvc');                                                
+                        
+                    case AttConsensusDecided(id, decided_attestation_data) => 
+                        lemma_inv17_f_att_consensus_decided(dvc, id, decided_attestation_data, dvc');                                                
+                        
+                    case ReceviedAttesttionShare(attestation_share) =>                         
+                        lemma_inv17_f_listen_for_attestation_shares(dvc, attestation_share, dvc');                        
+                       
+                    case ImportedNewBlock(block) => 
+                        var dvc_mod := add_block_to_bn(dvc, block);
+                        lemma_inv17_add_block_to_bn(dvc, block, dvc_mod);
+                        assert inv17_body(dvc_mod);
+                        lemma_inv17_f_listen_for_new_imported_blocks(dvc_mod, block, dvc');                        
+                        assert inv17_body(dvc');
+                    
+                    case ResendAttestationShares =>                                                                      
+
+                    case NoEvent => 
+                        
+                }
+                
+            case AdeversaryTakingStep(node, new_attestation_share_sent, messagesReceivedByTheNode) =>
+                
+        }   
+    }  
+
+    lemma lemma_inv18_dvn_next(
+        dvn: DVState,
+        event: DV.Event,
+        dvn': DVState
+    )    
+    requires NextEvent(dvn, event, dvn')  
+    requires inv1(dvn)  
+    requires inv2(dvn)  
+    requires inv4(dvn)
+    requires inv5(dvn)
+    requires inv7(dvn)
+    requires inv13(dvn)  
+    requires inv17(dvn)
+    requires inv18(dvn)
+    ensures inv18(dvn')
+    {        
+        match event 
+        {
+            case HonestNodeTakingStep(node, nodeEvent, nodeOutputs) =>
+                var dvc := dvn.honest_nodes_states[node];
+                var dvc' := dvn'.honest_nodes_states[node];
+                
+                
+                match nodeEvent
+                {
+                    case ServeAttstationDuty(attestation_duty) =>                                                                     
+                        
+                        assert inv14_body(dvc, attestation_duty); 
+                        assert inv15_body(dvc, attestation_duty);                                             
+                        lemma_inv18_f_serve_attestation_duty(dvc, attestation_duty, dvc');    
+                        
+                    case AttConsensusDecided(id, decided_attestation_data) => 
+                        lemma_inv18_f_att_consensus_decided(dvc, id, decided_attestation_data, dvc');                                                
+                        
+                    case ReceviedAttesttionShare(attestation_share) =>                         
+                        lemma_inv18_f_listen_for_attestation_shares(dvc, attestation_share, dvc');                        
+                       
+                    case ImportedNewBlock(block) =>                     
+                        var dvc_mod := add_block_to_bn(dvc, block);
+                        lemma_inv5_add_block_to_bn(dvc, block, dvc_mod);
+                        assert inv5_body(dvc_mod);
+                        lemma_inv17_add_block_to_bn(dvc, block, dvc_mod);
+                        assert inv17_body(dvc_mod);
+                        lemma_inv18_add_block_to_bn(dvc, block, dvc_mod);
+                        assert inv18_body(dvc_mod);
+
+                        lemma_inv18_f_listen_for_new_imported_blocks(dvc_mod, block, dvc');                        
+                        assert inv18_body(dvc');
+                    
+                    case ResendAttestationShares =>                                                                                      
+
+                    case NoEvent => 
+                        
+                }
+                
+            case AdeversaryTakingStep(node, new_attestation_share_sent, messagesReceivedByTheNode) =>
+                
+        }   
+    }  
+    
+}
