src/dvspec/dafny/att_spec_proofs/incomplete_proofs.dfy
@@ -6,7 +6,8 @@ include "../specification/dvn.dfy"
 include "../att_spec_proofs/inv.dfy"
 include "../att_spec_proofs/assump.dfy"
 include "../att_spec_proofs/fnc_inv.dfy"
-include "../att_spec_proofs/dvn_next_inv.dfy"
+include "../att_spec_proofs/dvn_next_invs_1_7.dfy"
+include "../att_spec_proofs/dvn_next_invs_8_18.dfy"
 include "../att_spec_proofs/helper_sets_lemmas.dfy"
 
 
@@ -20,16 +21,31 @@ module Incomplete_Proofs
     import opened DV
     import opened Att_Inv_With_Empty_Initial_Attestation_Slashing_DB    
     import opened Helper_Sets_Lemmas
-    import opened DVN_Next_Inv
+    import opened DVN_Next_Invs_1_7
+    import opened DVN_Next_Invs_8_18
     import opened Fnc_Inv    
 
-    lemma {:axiom} axiom_inv15(dvc: DVCNodeState)    
-    ensures inv15_body(dvc)
+    lemma {:axiom} axiom_inv18(dvc: DVCNodeState)    
+    ensures inv18_body(dvc)
+
+    
+     
+    
+
+     
+
+    
+
+    
 
     
     
+
     
 
+    
+
+    
     
 
     
