src/dvspec/dafny/att_spec_proofs/proofs_intermediate_steps.dfy
@@ -1,0 +1,162 @@
+include "../commons.dfy"
+include "../specification/dvc_spec.dfy"
+include "../specification/consensus.dfy"
+include "../specification/network.dfy"
+include "../specification/dvn.dfy"
+include "../att_spec_proofs/inv.dfy"
+include "../att_spec_proofs/assump.dfy"
+include "../att_spec_proofs/helper_sets_lemmas.dfy"
+
+
+module Proofs_Intermediate_Steps
+{
+    import opened Types 
+    import opened CommonFunctions
+    import opened ConsensusSpec
+    import opened NetworkSpec
+    import opened DVCNode_Spec
+    import opened DV
+    import opened Att_Inv_With_Empty_Initial_Attestation_Slashing_DB    
+    import opened Helper_Sets_Lemmas    
+    
+
+
+    
+
+    lemma lemma_inv2_inv53(dvn: DVState)
+    requires inv2(dvn)
+    ensures inv53(dvn)
+    { }
+        
+    lemma lemma_inv11_ind_inv(
+        dvn: DVState
+    )         
+    requires inv1(dvn)      
+    requires inv6(dvn)    
+    requires inv14(dvn)
+    ensures inv11(dvn)
+    {   
+        var queue := dvn.sequence_attestation_duties_to_be_served;
+        var index := dvn.index_next_attestation_duty_to_be_served;        
+        var next_duty := queue[index].attestation_duty;
+        var hn := queue[index].node;
+
+        if hn in dvn.honest_nodes_states.Keys 
+        {
+            var dvc := dvn.honest_nodes_states[hn];
+            if dvc.current_attestation_duty.isPresent()
+            {
+                var duty := dvc.current_attestation_duty.safe_get();
+                assert duty in dvc.all_rcvd_duties;  
+                assert duty.slot <= next_duty.slot;  
+            }
+        }
+    } 
+    
+    lemma lemma_inv12_ind_inv(
+        dvn: DVState
+    )         
+    requires inv1(dvn)      
+    requires inv7(dvn)    
+    requires inv14(dvn)
+    ensures inv12(dvn)
+    {   
+        var queue := dvn.sequence_attestation_duties_to_be_served;
+        var index := dvn.index_next_attestation_duty_to_be_served;        
+        var next_duty := queue[index].attestation_duty;
+        var hn := queue[index].node;
+
+        if hn in dvn.honest_nodes_states.Keys 
+        {
+            var dvc := dvn.honest_nodes_states[hn];
+            if dvc.latest_attestation_duty.isPresent()
+            {
+                var duty := dvc.latest_attestation_duty.safe_get();
+                assert duty in dvc.all_rcvd_duties;  
+                assert duty.slot <= next_duty.slot;  
+            }
+        }
+    } 
+      
+    lemma lemma_inv14_ind_inv(
+        dvn: DVState
+    )    
+    requires inv1(dvn)  
+    requires inv4(dvn)
+    requires inv13(dvn)
+    ensures inv14(dvn)    
+    {   
+        var queue := dvn.sequence_attestation_duties_to_be_served;
+        var index := dvn.index_next_attestation_duty_to_be_served;        
+        var next_duty := queue[index].attestation_duty;
+        var hn := queue[index].node;
+
+        if hn in dvn.honest_nodes_states.Keys 
+        {
+            var dvc := dvn.honest_nodes_states[hn];
+
+            assert inv4_body(dvn, hn, dvc);
+
+
+            forall rcvd_duty: AttestationDuty | rcvd_duty in dvc.all_rcvd_duties
+            ensures rcvd_duty.slot <= next_duty.slot
+            {
+                
+                var k: nat :| && 0 <= k < dvn.index_next_attestation_duty_to_be_served
+                              && dvn.sequence_attestation_duties_to_be_served[k].node == hn
+                              && dvn.sequence_attestation_duties_to_be_served[k].attestation_duty == rcvd_duty;
+
+                assert dvn.sequence_attestation_duties_to_be_served[k].attestation_duty.slot <= next_duty.slot;
+
+                assert rcvd_duty.slot <= next_duty.slot;
+            }
+
+            assert inv14_body(dvc, next_duty);
+            
+        }        
+    }
+
+    lemma lemma_inv15_ind_inv(
+        dvn: DVState
+    )    
+    requires inv1(dvn)  
+    requires inv4(dvn)
+    requires inv5(dvn)
+    requires inv13(dvn)
+    requires inv14(dvn)
+    ensures inv15(dvn)    
+    {   
+        var queue := dvn.sequence_attestation_duties_to_be_served;
+        var index := dvn.index_next_attestation_duty_to_be_served;        
+        var next_duty := queue[index].attestation_duty;
+        var hn := queue[index].node;
+
+        if hn in dvn.honest_nodes_states.Keys 
+        {
+            var dvc := dvn.honest_nodes_states[hn];
+
+            assert inv4_body(dvn, hn, dvc);
+            assert inv5_body(dvc);
+            assert inv14_body(dvc, next_duty);
+
+
+            forall queued_duty: AttestationDuty | queued_duty in dvc.attestation_duties_queue
+            ensures queued_duty.slot <= next_duty.slot
+            {
+                assert queued_duty in dvc.all_rcvd_duties;
+                
+                var k: nat :| && 0 <= k < dvn.index_next_attestation_duty_to_be_served
+                              && dvn.sequence_attestation_duties_to_be_served[k].node == hn
+                              && dvn.sequence_attestation_duties_to_be_served[k].attestation_duty == queued_duty;
+
+                assert dvn.sequence_attestation_duties_to_be_served[k].attestation_duty.slot <= next_duty.slot;
+
+                assert queued_duty.slot <= next_duty.slot;
+            }
+
+            assert inv15_body(dvc, next_duty);
+            
+        }        
+    }
+    
+}
